fixed bugs 1) memory allocated in C, say GenericValue, should be marked (CAMLparam, CAMLreturn) to prevent from being garbage collected by OCaml. 2) phinode list can also refer to constant, not only id; redefined 'switchToNewBasicBlock'. 3) in llvm2coq.ml, LLVM AST has a function type (rt typs)*, which should be separated into rt and list of typs in Coq AST; the @G in LLVM AST should be translated into (value_const (const_gid _ G)), rather than (value_id G), because (value_id id) only refers to locals. 4) some trivial bugs in Ocaml-llvm bindings
This version's ssa_main can interprete all integer insns and  memory operations
wrapped by Ocaml-llvm bindings, and functions. The next step is to
support float insns, gep and external functions.



git-svn-id: https://webdav.seas.upenn.edu/svn/sol/vol@2696 eef5ea85-cc2e-0410-bd84-0fae1f012da8

src/Parser/Output.ll
@@ -35,8 +35,8 @@ Loop:                                             ; preds = %Loop, %entry
   %nextindvar = add i32 %indvar, 1                ; <i32> [#uses=1]
   %5 = call i99 @ttt(i32* %0)                     ; <i99> [#uses=0]
   %6 = icmp eq i32 4, 5                           ; <i1> [#uses=0]
-  %x2 = load i32* %0, align 4                     ; <i32> [#uses=0]
-  %x1 = add i13 7, 8                              ; <i13> [#uses=0]
+  %x2 = add i13 7, 8                              ; <i13> [#uses=0]
+  %x1 = load i32* %0, align 4                     ; <i32> [#uses=0]
   br i1 false, label %Loop, label %return
 
 return:                                           ; preds = %Loop
